{
 "cells": [
  {
   "cell_type": "markdown",
   "metadata": {},
   "source": [
    "# Homework 1 - Credit Analytics\n",
    "Submission by Dennis Goldenberg"
   ]
  },
  {
   "cell_type": "markdown",
   "metadata": {},
   "source": [
    "## $\\text{\\underline{Question 1}}$"
   ]
  },
  {
   "cell_type": "markdown",
   "metadata": {},
   "source": [
    "### a. Proving $F(X) \\sim \\text{Uniform}(0,1)$\n",
    "Note that $F(x) = \\mathbb{P}(X \\leq x)$ and the support of a probability function is $S(\\mathbb{P}(\\cdot)) = (0,1]$. Therefore:\n",
    "$$\n",
    "\\begin{equation*}\n",
    "F(X) = \\mathbb{P}(X \\leq X) = 1 \\sim \\text{Uniform}(0,1)\n",
    "\\end{equation*}\n",
    "$$"
   ]
  },
  {
   "cell_type": "markdown",
   "metadata": {},
   "source": [
    "### b. Proving $F^{-1}(U) \\equiv X$\n",
    "Let $U \\sim \\text{Uniform}(0,1)$. Note that, via the definition of inverse function:\n",
    "$$\n",
    "\\begin{equation*}\n",
    "F^{-1}\\left(F(X)\\right) = X\n",
    "\\end{equation*}\n",
    "$$\n",
    "From a, $F(X) \\equiv U(0,1)$, so $F^{-1}\\left(U\\right) \\equiv F^{-1}\\left(F(X)\\right)$. So:\n",
    "$$\n",
    "\\begin{equation*}\n",
    "F^{-1}\\left(U\\right) \\equiv F^{-1}\\left(F(X)\\right) = X \\rightarrow F^{-1}\\left(U\\right) \\equiv X\n",
    "\\end{equation*}\n",
    "$$"
   ]
  },
  {
   "cell_type": "markdown",
   "metadata": {},
   "source": [
    "### c. Proving $\\Phi^{-1}(F(X)) \\equiv Y \\sim N(0,1)$\n",
    "From a, $F(X) \\equiv U(0,1)$. Note that $F(y) = \\Phi(y)$. Using the result from b:\n",
    "$$\n",
    "\\begin{equation*}\n",
    "\\Phi^{-1}(F(X)) \\equiv \\Phi^{-1}(U) = F_{Y}^{-1}(U) \\equiv Y\n",
    "\\end{equation*}\n",
    "$$\n",
    "Thus, $\\Phi^{-1}(F(X)) \\equiv Y \\sim N(0,1)$."
   ]
  },
  {
   "cell_type": "markdown",
   "metadata": {},
   "source": [
    "## $\\text{\\underline{Question 2}}$"
   ]
  },
  {
   "cell_type": "markdown",
   "metadata": {},
   "source": [
    "### a. Deriving survival function\n",
    "Note that, from a formula in class, $S(t) = \\mathbb{P}(\\tau > t) = e^{-\\int_0^{t}h(s)ds}$. Thus, I have:\n",
    "$$ \n",
    "\\begin{align*}\n",
    "S(t) = e^{-\\int_0^{t}\\alpha e^{\\beta s}ds} = e^{-\\alpha\\int_0^{t}e^{\\beta s}ds} &= e^{-\\alpha\\left[\\frac{1}{\\beta}e^{\\beta s}\\right]_{0}^{t}} = e^{-\\frac{\\alpha}{\\beta}\\left[e^{\\beta t} - 1\\right]} = e^{\\frac{\\alpha}{\\beta} - \\frac{\\alpha}{\\beta}e^{\\beta t}}\n",
    "\\end{align*}\n",
    "$$"
   ]
  },
  {
   "cell_type": "markdown",
   "metadata": {},
   "source": [
    "### b. Deriving the distribution function\n",
    "Using the fact that $S(t) = 1 - F(t) \\rightarrow F(t) + S(t) = 1 \\rightarrow F(t) = 1 - S(t)$, I compute:\n",
    "$$\n",
    "\\begin{equation*}\n",
    "F(t) = 1 - S(t)  = 1 - e^{\\frac{\\alpha}{\\beta} - \\frac{\\alpha}{\\beta}e^{\\beta t}} \n",
    "\\end{equation*}\n",
    "$$"
   ]
  },
  {
   "cell_type": "markdown",
   "metadata": {},
   "source": [
    "### c. Deriving the density function \n",
    "The density function is the derivative of the disrtibution function. I use this and apply the chain rule for derivatives:\n",
    "$$\n",
    "\\begin{align*}\n",
    "f(t) = \\frac{d}{dt}F(t) = \\frac{d}{dt}\\left(1 - e^{\\frac{\\alpha}{\\beta} - \\frac{\\alpha}{\\beta}e^{\\beta t}}\\right) &= -e^{\\frac{\\alpha}{\\beta}}\\frac{d}{dt}\\left(e^{-\\frac{\\alpha}{\\beta}e^{\\beta t}}\\right)\\\\\n",
    "&= -e^{\\frac{\\alpha}{\\beta}} * e^{-\\frac{\\alpha}{\\beta}e^{\\beta t}} * \\frac{d}{dt}\\left(-\\frac{\\alpha}{\\beta}e^{\\beta t}\\right)\\\\\n",
    "&= -e^{\\frac{\\alpha}{\\beta}} * e^{-\\frac{\\alpha}{\\beta}e^{\\beta t}} * -\\alpha e^{\\beta t}\\\\\n",
    "&= \\alpha e^{\\beta t +\\frac{\\alpha}{\\beta} - \\frac{\\alpha}{\\beta}e^{\\beta t}}\\\\\n",
    "&= \\alpha e^{\\beta t + \\frac{\\alpha}{\\beta}\\left(1 - e^{\\beta t}\\right)}\n",
    "\\end{align*}\n",
    "$$"
   ]
  },
  {
   "cell_type": "markdown",
   "metadata": {},
   "source": [
    "## $\\text{\\underline{Question 3}}$"
   ]
  },
  {
   "cell_type": "markdown",
   "metadata": {},
   "source": [
    "### a. Calculating Expected Value and Variance for Payout at Default\n",
    "Note that the probability of default at any specific time is given by the hazard function $h(t) = h$, as the hazard function is the probability of default conditional on survival up until that point. Further, since 100 dollars is paid out at time of default, and an instantaneous forward rate is $r(t) = r$, I calculate the discount factor from time $t$ back to to time 0 as:\n",
    "$$\n",
    "D(0,t) = e^{-\\int_0^{t}r(s)ds} = e^{-\\int_0^{t}rds} = e^{-rt}\n",
    "$$\n",
    "Thus, the present value of a contract that defaults at time $t$ is:\n",
    "$$\n",
    "PV(C|\\text{Default at time t}) = 100e^{-rt}\n",
    "$$\n",
    "The payout for no default is 0, so this does not have to be discounted to the present, as it will still be 0. Therefore, I calculate the expected value:\n",
    "$$\n",
    "\\begin{align*}\n",
    "\\mathbb{E}[PV(C)] = \\int_0^{T}PV_t(C)*\\mathbb{P}(\\text{default at }t)dt &= \\int_0^{T}100e^{-rt}*hdt\\\\\n",
    "&= 100h\\int_0^{T}e^{-rt}dt\\\\\n",
    "&= 100h\\left[\\frac{-1}{r}e^{-rt}\\right]_0^T\\\\\n",
    "&= \\frac{100h}{r}\\left(1 - e^{-rT}\\right)\n",
    "\\end{align*}\n",
    "$$\n",
    "For variance, I use a common relation of variance to calculate:\n",
    "$$\n",
    "\\begin{align*}\n",
    "Var[PV(C)] = \\mathbb{E}[PV(C)^2] - \\mathbb{E}[PV(C)]^2 &= \\int_0^{T}PV_t(C)^2*\\mathbb{P}(\\text{default at }t)dt - \\left(\\frac{100h}{r}\\left(1 - e^{-rT}\\right)\\right)^2\\\\\n",
    "&= \\int_0^{T}\\left(100e^{-rt}\\right)^2*h dt - \\frac{10,000h^2}{r^2}\\left(1 - e^{-rT}\\right)^2\\\\\n",
    "&= 10,000h\\int_0^{T}e^{-2rt}dt - \\frac{10,000h^2}{r^2}\\left(1 - e^{-rT}\\right)^2\\\\\n",
    "&= 10,000h\\left[\\frac{-1}{2r}e^{-2rt}\\right]_0^{T} - \\frac{10,000h^2}{r^2}\\left(1 - e^{-rT}\\right)^2\\\\\n",
    "&= 10,000h * \\frac{1}{2r}\\left(1 - e^{-2rT}\\right)- \\frac{10,000h^2}{r^2}\\left(1 - e^{-rT}\\right)^2\\\\\n",
    "&= \\frac{5,000h}{r}\\left(1 - e^{-2rT}\\right) - \\frac{10,000h^2}{r^2}\\left(1 - e^{-rT}\\right)^2\\\\\n",
    "&= \\frac{5,000h}{r}\\left(1 - e^{-rT}\\right)\\left(1 + e^{-rT}\\right) - \\frac{10,000h^2}{r^2}\\left(1 - e^{-rT}\\right)^2\\\\\n",
    "&= \\frac{5000h}{r}\\left(1 - e^{-rT}\\right)\\left(1 + e^{-rT} - \\frac{2h}{r}\\left(1 - e^{-rT}\\right)\\right)\n",
    "\\end{align*}\n",
    "$$"
   ]
  },
  {
   "cell_type": "markdown",
   "metadata": {},
   "source": [
    "### b. Calculate Expected Value, Variance for Payout if No Default\n",
    " "
   ]
  },
  {
   "cell_type": "code",
   "execution_count": 5,
   "metadata": {},
   "outputs": [],
   "source": [
    "import pandas as pd"
   ]
  },
  {
   "cell_type": "code",
   "execution_count": 3,
   "metadata": {},
   "outputs": [
    {
     "data": {
      "text/plain": [
       "2.0"
      ]
     },
     "execution_count": 3,
     "metadata": {},
     "output_type": "execute_result"
    }
   ],
   "source": []
  }
 ],
 "metadata": {
  "kernelspec": {
   "display_name": ".venv",
   "language": "python",
   "name": "python3"
  },
  "language_info": {
   "codemirror_mode": {
    "name": "ipython",
    "version": 3
   },
   "file_extension": ".py",
   "mimetype": "text/x-python",
   "name": "python",
   "nbconvert_exporter": "python",
   "pygments_lexer": "ipython3",
   "version": "3.11.7"
  }
 },
 "nbformat": 4,
 "nbformat_minor": 2
}
